Ex.Intro: Add effect to lib (but not yet to callback)

state/Examples.Intro.fst
@@ -9,17 +9,23 @@ open FStar.Tactics.Typeclasses
 open SharedRefs
 open Witnessable
 
-// TODO: Make lib effectful
-let prog (lib : (ref (ref int) -> cb:(unit -> unit))) : SST unit (requires fun h0 -> True) (ensures fun h0 _ h1 -> True) =
+type lib_type =
+  ref (ref int) -> SST (unit -> unit) (fun _ -> True) (fun _ _ _ -> True)
+
+let prog (lib : lib_type) : SST unit (requires fun h0 -> True) (ensures fun h0 _ h1 -> True) =
   let secret : ref int = sst_alloc 42 in
   let r : ref (ref int) = sst_alloc_shared #(SRef SNat) (sst_alloc_shared #(SNat) 0) in
+  assert (!secret == 42);
   let cb = lib r in
+  assume (!secret == 42);
   // r := sst_alloc_shared #(SNat) 1;
   let v : ref int = sst_alloc_shared #(SNat) 1 in
-  assume (forall h0. (forall (t: shareable_typ).
+  let h = get_heap () in
+  assume (forall (t: shareable_typ).
               to_Type t == ref int ==>
-              forall_refs_heap contains_pred h0 #t v /\
-              (is_shared r h0 ==> forall_refs_heap is_shared h0 #t v))) ;
+              forall_refs_heap contains_pred h #t v /\
+              (is_shared r h ==> forall_refs_heap is_shared h #t v)) ;
   sst_write_ref r v;
+  assert (!secret == 42);
   cb ();
   assert (!secret == 42)
